-

src/Structures.v
@@ -392,6 +392,24 @@ Arguments rngl_abs {T ro} a%_L.
 
 Notation "∣ x ∣" := (rngl_abs x) (at level 35, x at level 30).
 
+Definition rngl_has_inv_and_1_or_divl_comm_or_divr T {ro : ring_like_op T}
+  {rp : ring_like_prop T} :=
+  match rngl_opt_inv_or_pdiv T with
+  | Some (inl _) => rngl_has_1 T
+  | Some (inr (inl _)) => rngl_mul_is_comm T
+  | Some (inr (inr _)) => true
+  | None => false
+  end.
+
+Definition rngl_has_inv_and_1_or_divl_or_divr_comm T {ro : ring_like_op T}
+  {rp : ring_like_prop T} :=
+  match rngl_opt_inv_or_pdiv T with
+  | Some (inl _) => rngl_has_1 T
+  | Some (inr (inl _)) => true
+  | Some (inr (inr _)) => rngl_mul_is_comm T
+  | None => false
+  end.
+
 Section a.
 
 Context {T : Type}.
